Lean4Lean/TypeChecker.lean
@@ -288,8 +288,7 @@ def whnfFVar (e : Expr) (cheapRec cheapProj : Bool) : RecM Expr := do
     return ← whnfCore v cheapRec cheapProj
   return e
 
-def reduceProj (typeName : Name) (idx : Nat) (struct : Expr)
-    (cheapRec cheapProj : Bool) : RecM (Option Expr) := do
+def reduceProj (idx : Nat) (struct : Expr) (cheapRec cheapProj : Bool) : RecM (Option Expr) := do
   let mut c ← (if cheapProj then whnfCore struct cheapRec cheapProj else whnf struct)
   if let .lit (.strVal s) := c then
     c ← whnf (.strLitToConstructor s)
@@ -297,7 +296,6 @@ def reduceProj (typeName : Name) (idx : Nat) (struct : Expr)
   let .const mkC _ := mk | return none
   let env ← getEnv
   let .ctorInfo mkInfo ← env.get mkC | return none
-  if mkInfo.induct != typeName then return none
   return args[mkInfo.numParams + idx]?
 
 def isLetFVar (lctx : LocalContext) (fvar : FVarId) : Bool :=
@@ -343,8 +341,8 @@ def whnfCore' (e : Expr) (cheapRec := false) (cheapProj := false) : RecM Expr :=
       save <|← whnfCore r cheapRec cheapProj
   | .letE _ _ val body _ =>
     save <|← whnfCore (body.instantiate1 val) cheapRec cheapProj
-  | .proj typeName idx s =>
-    if let some m ← reduceProj typeName idx s cheapRec cheapProj then
+  | .proj _ idx s =>
+    if let some m ← reduceProj idx s cheapRec cheapProj then
       save <|← whnfCore m cheapRec cheapProj
     else
       save e
@@ -692,8 +690,8 @@ def isDefEqCore' (t s : Expr) : RecM Bool := do
   | .const tf tl, .const sf sl =>
     if tf == sf && Level.isEquivList tl sl then return true
   | .fvar tv, .fvar sv => if tv == sv then return true
-  | .proj tStruct ti te, .proj sStruct si se =>
-    if tStruct == sStruct && ti == si then if ← isDefEq te se then return true
+  | .proj _ ti te, .proj _ si se =>
+    if ti == si then if ← isDefEq te se then return true
   | _, _ => pure ()
 
   let tnn ← whnfCore tn
